Instructions + properties file

src/bin/test.cs
@@ -1,0 +1,2303 @@
+// Dafny program test.dfy compiled into C#
+// To recompile, you will need the libraries
+//     System.Runtime.Numerics.dll System.Collections.Immutable.dll
+// but the 'dotnet' tool in net5.0 should pick those up automatically.
+// Optionally, you may want to include compiler switches like
+//     /debug /nowarn:162,164,168,183,219,436,1717,1718
+
+using System;
+using System.Numerics;
+[assembly: DafnyAssembly.DafnySourceAttribute(@"// Dafny 3.3.0.31104
+// Command Line Options: /home/alexis51151/Ecole/Rice University/COMP-517/comp517-project/src/dafny/test.dfy /verifyAllModules /spillTargetCode:1 /compile:3 /out:bin/test
+// test.dfy
+
+class Test {
+  method testProcess1()
+  {
+    var kernel: Kernel := new Kernel();
+    var endokernel: Endokernel := new Endokernel(kernel);
+    var instruction: Instruction := Write('a', 0);
+    var thread: Thread := new Thread(0, 0, 0, [instruction], endokernel);
+    var p: Process := new Process(0, [0, 1, 2, 3], endokernel, thread);
+    p.exec();
+  }
+
+  method Main()
+  {
+    testProcess1();
+  }
+}
+
+class Process {
+  var pid: int
+  var memorySpace: seq<int>
+  var endokernel: Endokernel
+  var thread: Thread
+
+  constructor (pid: int, memorySpace: seq<int>, endokernel_: Endokernel, thread_: Thread)
+    ensures this.endokernel == old(endokernel_)
+    ensures this.thread == old(thread_)
+    decreases pid, memorySpace, endokernel_, thread_
+  {
+    this.pid := pid;
+    this.memorySpace := memorySpace;
+    this.endokernel := endokernel_;
+    this.thread := thread_;
+  }
+
+  method exec()
+    modifies this, thread, thread.endokernel
+  {
+    thread.exec();
+  }
+}
+
+class Endokernel {
+  var capabilities: map<Capability, Endoprocess>
+  var endoprocesses: map<int, Endoprocess>
+  var instructionMap: map<Instruction, Capability>
+  var nextPid: int
+  var kernel: Kernel
+
+  method createEndoprocess(capability: Capability, instruction: Instruction) returns (endoprocess: Endoprocess)
+    modifies this
+    decreases capability, instruction
+  {
+    endoprocess := new Endoprocess(this.nextPid, capability.subspace, instruction, this);
+    this.capabilities := capabilities[capability := endoprocess];
+    this.endoprocesses := this.endoprocesses[this.nextPid := endoprocess];
+    this.nextPid := nextPid + 1;
+  }
+
+  method trap(instruction: Instruction)
+    modifies this
+    decreases instruction
+  {
+    if instruction !in instructionMap {
+      print ""trap error: no policy for this instruction\n"";
+    } else {
+      var capability: Capability := instructionMap[instruction];
+      var endoprocess: Endoprocess;
+      if capability !in capabilities {
+        endoprocess := createEndoprocess(capability, instruction);
+      } else {
+        endoprocess := capabilities[capability];
+      }
+      print ""Trapping instruction"";
+      print instruction;
+      print ""from Process in Endokernel\n"";
+      endoprocess.exec(instruction);
+    }
+  }
+
+  method trapEndoprocess(instruction: Instruction, endoId: int)
+    decreases instruction, endoId
+  {
+    if instruction !in instructionMap {
+      print ""trapEndoprocess error: no policy for this instruction\n"";
+    } else {
+      var capability := instructionMap[instruction];
+      if capability !in capabilities {
+        print ""trapEndoprocess error: this endoprocess has not the required rights for such instruction\n"";
+      } else {
+        var endoprocessExpected := capabilities[capability];
+        if endoId !in endoprocesses {
+          print ""trapEndoprocess error: unknown endoprocess\n"";
+        } else {
+          var endoprocessTrapped := endoprocesses[endoId];
+          if endoprocessTrapped != endoprocessExpected {
+            print ""trapEndoprocess error: unknown endoprocess\n"";
+          } else {
+            print ""Trapping back instruction from Endoprocess in Endokernel\n"";
+            kernel.exec(instruction);
+          }
+        }
+      }
+    }
+  }
+
+  constructor (kernel: Kernel)
+    decreases kernel
+  {
+    this.nextPid := 0;
+    this.capabilities := map[];
+    this.endoprocesses := map[];
+    var capability: Capability := new Capability();
+    var instruction: Instruction := Write('a', 0);
+    this.instructionMap := map[instruction := capability];
+    this.kernel := kernel;
+  }
+}
+
+class Endoprocess {
+  var id: int
+  var memorySpace: seq<int>
+  var instructions: Instruction
+  var endokernel: Endokernel
+
+  constructor (id: int, memorySpace: seq<int>, instructions: Instruction, endokernel: Endokernel)
+    decreases id, memorySpace, instructions, endokernel
+  {
+    this.id := id;
+    this.memorySpace := memorySpace;
+    this.instructions := instructions;
+    this.endokernel := endokernel;
+  }
+
+  method exec(instruction: Instruction)
+    decreases instruction
+  {
+    print ""Executing instruction in Endoprocess\n"";
+    endokernel.trapEndoprocess(instruction, this.id);
+  }
+}
+
+class Kernel {
+  method exec(instruction: Instruction)
+    decreases instruction
+  {
+    print ""Executing instruction in kernel\n"";
+  }
+
+  constructor ()
+  {
+  }
+}
+
+class Thread {
+  var tid: int
+  var pc: int
+  var sp: int
+  var instructions: seq<Instruction>
+  var endokernel: Endokernel
+
+  constructor (tid: int, pc: int, sp: int, instructions: seq<Instruction>, endokernel: Endokernel)
+    ensures this.endokernel == old(endokernel)
+    decreases tid, pc, sp, instructions, endokernel
+  {
+    this.tid := tid;
+    this.pc := pc;
+    this.sp := sp;
+    this.instructions := instructions;
+    this.endokernel := endokernel;
+  }
+
+  method exec()
+    modifies this, endokernel
+  {
+    if 0 <= pc < |instructions| {
+      print ""Executing instruction in Process\n"";
+      this.endokernel.trap(instructions[pc]);
+      pc := pc + 1;
+    }
+  }
+}
+
+datatype Instruction = Write(value: char, addr: int) | Read(addr: int)
+
+class Capability {
+  var subspace: seq<int>
+  var stack: seq<int>
+  var files: seq<string>
+  var entries: seq<string>
+
+  constructor ()
+  {
+    subspace := [];
+    stack := [];
+    files := [];
+    entries := [];
+  }
+}
+")]
+
+//-----------------------------------------------------------------------------
+//
+// Copyright by the contributors to the Dafny Project
+// SPDX-License-Identifier: MIT
+//
+//-----------------------------------------------------------------------------
+
+#if ISDAFNYRUNTIMELIB
+using System; // for Func
+using System.Numerics;
+#endif
+
+namespace DafnyAssembly {
+  [AttributeUsage(AttributeTargets.Assembly)]
+  public class DafnySourceAttribute : Attribute {
+    public readonly string dafnySourceText;
+    public DafnySourceAttribute(string txt) { dafnySourceText = txt; }
+  }
+}
+
+namespace Dafny {
+  using System.Collections.Generic;
+  using System.Collections.Immutable;
+  using System.Linq;
+
+  public interface ISet<out T> {
+    int Count { get; }
+    long LongCount { get; }
+    IEnumerable<T> Elements { get; }
+    IEnumerable<ISet<T>> AllSubsets { get; }
+    bool Contains<G>(G t);
+    bool EqualsAux(ISet<object> other);
+    ISet<U> DowncastClone<U>(Func<T, U> converter);
+  }
+
+  public class Set<T> : ISet<T> {
+    readonly ImmutableHashSet<T> setImpl;
+    readonly bool containsNull;
+    Set(ImmutableHashSet<T> d, bool containsNull) {
+      this.setImpl = d;
+      this.containsNull = containsNull;
+    }
+
+    public static readonly ISet<T> Empty = new Set<T>(ImmutableHashSet<T>.Empty, false);
+
+    private static readonly TypeDescriptor<ISet<T>> _TYPE = new Dafny.TypeDescriptor<ISet<T>>(Empty);
+    public static TypeDescriptor<ISet<T>> _TypeDescriptor() {
+      return _TYPE;
+    }
+
+    public static ISet<T> FromElements(params T[] values) {
+      return FromCollection(values);
+    }
+
+    public static Set<T> FromISet(ISet<T> s) {
+      return s as Set<T> ?? FromCollection(s.Elements);
+    }
+
+    public static Set<T> FromCollection(IEnumerable<T> values) {
+      var d = ImmutableHashSet<T>.Empty.ToBuilder();
+      var containsNull = false;
+      foreach (T t in values) {
+        if (t == null) {
+          containsNull = true;
+        } else {
+          d.Add(t);
+        }
+      }
+
+      return new Set<T>(d.ToImmutable(), containsNull);
+    }
+
+    public static ISet<T> FromCollectionPlusOne(IEnumerable<T> values, T oneMoreValue) {
+      var d = ImmutableHashSet<T>.Empty.ToBuilder();
+      var containsNull = false;
+      if (oneMoreValue == null) {
+        containsNull = true;
+      } else {
+        d.Add(oneMoreValue);
+      }
+
+      foreach (T t in values) {
+        if (t == null) {
+          containsNull = true;
+        } else {
+          d.Add(t);
+        }
+      }
+
+      return new Set<T>(d.ToImmutable(), containsNull);
+    }
+
+    public ISet<U> DowncastClone<U>(Func<T, U> converter) {
+      if (this is ISet<U> th) {
+        return th;
+      } else {
+        var d = ImmutableHashSet<U>.Empty.ToBuilder();
+        foreach (var t in this.setImpl) {
+          var u = converter(t);
+          d.Add(u);
+        }
+
+        return new Set<U>(d.ToImmutable(), this.containsNull);
+      }
+    }
+
+    public int Count {
+      get { return this.setImpl.Count + (containsNull ? 1 : 0); }
+    }
+
+    public long LongCount {
+      get { return this.setImpl.Count + (containsNull ? 1 : 0); }
+    }
+
+    public IEnumerable<T> Elements {
+      get {
+        if (containsNull) {
+          yield return default(T);
+        }
+
+        foreach (var t in this.setImpl) {
+          yield return t;
+        }
+      }
+    }
+
+    /// <summary>
+    /// This is an inefficient iterator for producing all subsets of "this".
+    /// </summary>
+    public IEnumerable<ISet<T>> AllSubsets {
+      get {
+        // Start by putting all set elements into a list, but don't include null
+        var elmts = new List<T>();
+        elmts.AddRange(this.setImpl);
+        var n = elmts.Count;
+        var which = new bool[n];
+        var s = ImmutableHashSet<T>.Empty.ToBuilder();
+        while (true) {
+          // yield both the subset without null and, if null is in the original set, the subset with null included
+          var ihs = s.ToImmutable();
+          yield return new Set<T>(ihs, false);
+          if (containsNull) {
+            yield return new Set<T>(ihs, true);
+          }
+
+          // "add 1" to "which", as if doing a carry chain.  For every digit changed, change the membership of the corresponding element in "s".
+          int i = 0;
+          for (; i < n && which[i]; i++) {
+            which[i] = false;
+            s.Remove(elmts[i]);
+          }
+
+          if (i == n) {
+            // we have cycled through all the subsets
+            break;
+          }
+
+          which[i] = true;
+          s.Add(elmts[i]);
+        }
+      }
+    }
+
+    public bool Equals(ISet<T> other) {
+      if (other == null || Count != other.Count) {
+        return false;
+      } else if (this == other) {
+        return true;
+      }
+
+      foreach (var elmt in Elements) {
+        if (!other.Contains(elmt)) {
+          return false;
+        }
+      }
+
+      return true;
+    }
+
+    public override bool Equals(object other) {
+      if (other is ISet<T>) {
+        return Equals((ISet<T>)other);
+      }
+
+      var th = this as ISet<object>;
+      var oth = other as ISet<object>;
+      if (th != null && oth != null) {
+        // We'd like to obtain the more specific type parameter U for oth's type ISet<U>.
+        // We do that by making a dynamically dispatched call, like:
+        //     oth.Equals(this)
+        // The hope is then that its comparison "this is ISet<U>" (that is, the first "if" test
+        // above, but in the call "oth.Equals(this)") will be true and the non-virtual Equals
+        // can be called. However, such a recursive call to "oth.Equals(this)" could turn
+        // into infinite recursion. Therefore, we instead call "oth.EqualsAux(this)", which
+        // performs the desired type test, but doesn't recurse any further.
+        return oth.EqualsAux(th);
+      } else {
+        return false;
+      }
+    }
+
+    public bool EqualsAux(ISet<object> other) {
+      var s = other as ISet<T>;
+      if (s != null) {
+        return Equals(s);
+      } else {
+        return false;
+      }
+    }
+
+    public override int GetHashCode() {
+      var hashCode = 1;
+      if (containsNull) {
+        hashCode = hashCode * (Dafny.Helpers.GetHashCode(default(T)) + 3);
+      }
+
+      foreach (var t in this.setImpl) {
+        hashCode = hashCode * (Dafny.Helpers.GetHashCode(t) + 3);
+      }
+
+      return hashCode;
+    }
+
+    public override string ToString() {
+      var s = "{";
+      var sep = "";
+      if (containsNull) {
+        s += sep + Dafny.Helpers.ToString(default(T));
+        sep = ", ";
+      }
+
+      foreach (var t in this.setImpl) {
+        s += sep + Dafny.Helpers.ToString(t);
+        sep = ", ";
+      }
+
+      return s + "}";
+    }
+    public static bool IsProperSubsetOf(ISet<T> th, ISet<T> other) {
+      return th.Count < other.Count && IsSubsetOf(th, other);
+    }
+    public static bool IsSubsetOf(ISet<T> th, ISet<T> other) {
+      if (other.Count < th.Count) {
+        return false;
+      }
+      foreach (T t in th.Elements) {
+        if (!other.Contains(t)) {
+          return false;
+        }
+      }
+      return true;
+    }
+    public static bool IsDisjointFrom(ISet<T> th, ISet<T> other) {
+      ISet<T> a, b;
+      if (th.Count < other.Count) {
+        a = th; b = other;
+      } else {
+        a = other; b = th;
+      }
+      foreach (T t in a.Elements) {
+        if (b.Contains(t)) {
+          return false;
+        }
+      }
+      return true;
+    }
+    public bool Contains<G>(G t) {
+      return t == null ? containsNull : t is T && this.setImpl.Contains((T)(object)t);
+    }
+    public static ISet<T> Union(ISet<T> th, ISet<T> other) {
+      var a = FromISet(th);
+      var b = FromISet(other);
+      return new Set<T>(a.setImpl.Union(b.setImpl), a.containsNull || b.containsNull);
+    }
+    public static ISet<T> Intersect(ISet<T> th, ISet<T> other) {
+      var a = FromISet(th);
+      var b = FromISet(other);
+      return new Set<T>(a.setImpl.Intersect(b.setImpl), a.containsNull && b.containsNull);
+    }
+    public static ISet<T> Difference(ISet<T> th, ISet<T> other) {
+      var a = FromISet(th);
+      var b = FromISet(other);
+      return new Set<T>(a.setImpl.Except(b.setImpl), a.containsNull && !b.containsNull);
+    }
+  }
+
+  public interface IMultiSet<out T> {
+    bool IsEmpty { get; }
+    int Count { get; }
+    long LongCount { get; }
+    IEnumerable<T> Elements { get; }
+    IEnumerable<T> UniqueElements { get; }
+    bool Contains<G>(G t);
+    BigInteger Select<G>(G t);
+    IMultiSet<T> Update<G>(G t, BigInteger i);
+    bool EqualsAux(IMultiSet<object> other);
+    IMultiSet<U> DowncastClone<U>(Func<T, U> converter);
+  }
+
+  public class MultiSet<T> : IMultiSet<T> {
+    readonly ImmutableDictionary<T, BigInteger> dict;
+    readonly BigInteger occurrencesOfNull;  // stupidly, a Dictionary in .NET cannot use "null" as a key
+    MultiSet(ImmutableDictionary<T, BigInteger>.Builder d, BigInteger occurrencesOfNull) {
+      dict = d.ToImmutable();
+      this.occurrencesOfNull = occurrencesOfNull;
+    }
+    public static readonly MultiSet<T> Empty = new MultiSet<T>(ImmutableDictionary<T, BigInteger>.Empty.ToBuilder(), BigInteger.Zero);
+
+    private static readonly TypeDescriptor<IMultiSet<T>> _TYPE = new Dafny.TypeDescriptor<IMultiSet<T>>(Empty);
+    public static TypeDescriptor<IMultiSet<T>> _TypeDescriptor() {
+      return _TYPE;
+    }
+
+    public static MultiSet<T> FromIMultiSet(IMultiSet<T> s) {
+      return s as MultiSet<T> ?? FromCollection(s.Elements);
+    }
+    public static MultiSet<T> FromElements(params T[] values) {
+      var d = ImmutableDictionary<T, BigInteger>.Empty.ToBuilder();
+      var occurrencesOfNull = BigInteger.Zero;
+      foreach (T t in values) {
+        if (t == null) {
+          occurrencesOfNull++;
+        } else {
+          BigInteger i;
+          if (!d.TryGetValue(t, out i)) {
+            i = BigInteger.Zero;
+          }
+          d[t] = i + 1;
+        }
+      }
+      return new MultiSet<T>(d, occurrencesOfNull);
+    }
+
+    public static MultiSet<T> FromCollection(IEnumerable<T> values) {
+      var d = ImmutableDictionary<T, BigInteger>.Empty.ToBuilder();
+      var occurrencesOfNull = BigInteger.Zero;
+      foreach (T t in values) {
+        if (t == null) {
+          occurrencesOfNull++;
+        } else {
+          BigInteger i;
+          if (!d.TryGetValue(t,
+            out i)) {
+            i = BigInteger.Zero;
+          }
+
+          d[t] = i + 1;
+        }
+      }
+
+      return new MultiSet<T>(d,
+        occurrencesOfNull);
+    }
+
+    public static MultiSet<T> FromSeq(ISequence<T> values) {
+      var d = ImmutableDictionary<T, BigInteger>.Empty.ToBuilder();
+      var occurrencesOfNull = BigInteger.Zero;
+      foreach (T t in values.Elements) {
+        if (t == null) {
+          occurrencesOfNull++;
+        } else {
+          BigInteger i;
+          if (!d.TryGetValue(t,
+            out i)) {
+            i = BigInteger.Zero;
+          }
+
+          d[t] = i + 1;
+        }
+      }
+
+      return new MultiSet<T>(d,
+        occurrencesOfNull);
+    }
+    public static MultiSet<T> FromSet(ISet<T> values) {
+      var d = ImmutableDictionary<T, BigInteger>.Empty.ToBuilder();
+      var containsNull = false;
+      foreach (T t in values.Elements) {
+        if (t == null) {
+          containsNull = true;
+        } else {
+          d[t] = BigInteger.One;
+        }
+      }
+      return new MultiSet<T>(d, containsNull ? BigInteger.One : BigInteger.Zero);
+    }
+    public IMultiSet<U> DowncastClone<U>(Func<T, U> converter) {
+      if (this is IMultiSet<U> th) {
+        return th;
+      } else {
+        var d = ImmutableDictionary<U, BigInteger>.Empty.ToBuilder();
+        foreach (var item in this.dict) {
+          var k = converter(item.Key);
+          d.Add(k, item.Value);
+        }
+        return new MultiSet<U>(d, this.occurrencesOfNull);
+      }
+    }
+
+    public bool Equals(IMultiSet<T> other) {
+      return IsSubsetOf(this, other) && IsSubsetOf(other, this);
+    }
+    public override bool Equals(object other) {
+      if (other is IMultiSet<T>) {
+        return Equals((IMultiSet<T>)other);
+      }
+      var th = this as IMultiSet<object>;
+      var oth = other as IMultiSet<object>;
+      if (th != null && oth != null) {
+        // See comment in Set.Equals
+        return oth.EqualsAux(th);
+      } else {
+        return false;
+      }
+    }
+
+    public bool EqualsAux(IMultiSet<object> other) {
+      var s = other as IMultiSet<T>;
+      if (s != null) {
+        return Equals(s);
+      } else {
+        return false;
+      }
+    }
+
+    public override int GetHashCode() {
+      var hashCode = 1;
+      if (occurrencesOfNull > 0) {
+        var key = Dafny.Helpers.GetHashCode(default(T));
+        key = (key << 3) | (key >> 29) ^ occurrencesOfNull.GetHashCode();
+        hashCode = hashCode * (key + 3);
+      }
+      foreach (var kv in dict) {
+        var key = Dafny.Helpers.GetHashCode(kv.Key);
+        key = (key << 3) | (key >> 29) ^ kv.Value.GetHashCode();
+        hashCode = hashCode * (key + 3);
+      }
+      return hashCode;
+    }
+    public override string ToString() {
+      var s = "multiset{";
+      var sep = "";
+      for (var i = BigInteger.Zero; i < occurrencesOfNull; i++) {
+        s += sep + Dafny.Helpers.ToString(default(T));
+        sep = ", ";
+      }
+      foreach (var kv in dict) {
+        var t = Dafny.Helpers.ToString(kv.Key);
+        for (var i = BigInteger.Zero; i < kv.Value; i++) {
+          s += sep + t;
+          sep = ", ";
+        }
+      }
+      return s + "}";
+    }
+    public static bool IsProperSubsetOf(IMultiSet<T> th, IMultiSet<T> other) {
+      return th.Count < other.Count && IsSubsetOf(th, other);
+    }
+    public static bool IsSubsetOf(IMultiSet<T> th, IMultiSet<T> other) {
+      var a = FromIMultiSet(th);
+      var b = FromIMultiSet(other);
+      if (b.occurrencesOfNull < a.occurrencesOfNull) {
+        return false;
+      }
+      foreach (T t in a.dict.Keys) {
+        if (b.dict.ContainsKey(t)) {
+          if (b.dict[t] < a.dict[t]) {
+            return false;
+          }
+        } else {
+          if (a.dict[t] != BigInteger.Zero) {
+            return false;
+          }
+        }
+      }
+      return true;
+    }
+    public static bool IsDisjointFrom(IMultiSet<T> th, IMultiSet<T> other) {
+      foreach (T t in th.UniqueElements) {
+        if (other.Contains(t)) {
+          return false;
+        }
+      }
+      return true;
+    }
+
+    public bool Contains<G>(G t) {
+      return Select(t) != 0;
+    }
+    public BigInteger Select<G>(G t) {
+      if (t == null) {
+        return occurrencesOfNull;
+      }
+      BigInteger m;
+      if (t is T && dict.TryGetValue((T)(object)t, out m)) {
+        return m;
+      } else {
+        return BigInteger.Zero;
+      }
+    }
+    public IMultiSet<T> Update<G>(G t, BigInteger i) {
+      if (Select(t) == i) {
+        return this;
+      } else if (t == null) {
+        var r = dict.ToBuilder();
+        return new MultiSet<T>(r, i);
+      } else {
+        var r = dict.ToBuilder();
+        r[(T)(object)t] = i;
+        return new MultiSet<T>(r, occurrencesOfNull);
+      }
+    }
+    public static IMultiSet<T> Union(IMultiSet<T> th, IMultiSet<T> other) {
+      if (th.IsEmpty) {
+        return other;
+      } else if (other.IsEmpty) {
+        return th;
+      }
+      var a = FromIMultiSet(th);
+      var b = FromIMultiSet(other);
+      var r = ImmutableDictionary<T, BigInteger>.Empty.ToBuilder();
+      foreach (T t in a.dict.Keys) {
+        BigInteger i;
+        if (!r.TryGetValue(t, out i)) {
+          i = BigInteger.Zero;
+        }
+        r[t] = i + a.dict[t];
+      }
+      foreach (T t in b.dict.Keys) {
+        BigInteger i;
+        if (!r.TryGetValue(t, out i)) {
+          i = BigInteger.Zero;
+        }
+        r[t] = i + b.dict[t];
+      }
+      return new MultiSet<T>(r, a.occurrencesOfNull + b.occurrencesOfNull);
+    }
+    public static IMultiSet<T> Intersect(IMultiSet<T> th, IMultiSet<T> other) {
+      if (th.IsEmpty) {
+        return th;
+      } else if (other.IsEmpty) {
+        return other;
+      }
+      var a = FromIMultiSet(th);
+      var b = FromIMultiSet(other);
+      var r = ImmutableDictionary<T, BigInteger>.Empty.ToBuilder();
+      foreach (T t in a.dict.Keys) {
+        if (b.dict.ContainsKey(t)) {
+          r.Add(t, a.dict[t] < b.dict[t] ? a.dict[t] : b.dict[t]);
+        }
+      }
+      return new MultiSet<T>(r, a.occurrencesOfNull < b.occurrencesOfNull ? a.occurrencesOfNull : b.occurrencesOfNull);
+    }
+    public static IMultiSet<T> Difference(IMultiSet<T> th, IMultiSet<T> other) { // \result == this - other
+      if (other.IsEmpty) {
+        return th;
+      }
+      var a = FromIMultiSet(th);
+      var b = FromIMultiSet(other);
+      var r = ImmutableDictionary<T, BigInteger>.Empty.ToBuilder();
+      foreach (T t in a.dict.Keys) {
+        if (!b.dict.ContainsKey(t)) {
+          r.Add(t, a.dict[t]);
+        } else if (b.dict[t] < a.dict[t]) {
+          r.Add(t, a.dict[t] - b.dict[t]);
+        }
+      }
+      return new MultiSet<T>(r, b.occurrencesOfNull < a.occurrencesOfNull ? a.occurrencesOfNull - b.occurrencesOfNull : BigInteger.Zero);
+    }
+
+    public bool IsEmpty { get { return occurrencesOfNull == 0 && dict.IsEmpty; } }
+
+    public int Count {
+      get { return (int)ElementCount(); }
+    }
+    public long LongCount {
+      get { return (long)ElementCount(); }
+    }
+    private BigInteger ElementCount() {
+      // This is inefficient
+      var c = occurrencesOfNull;
+      foreach (var item in dict) {
+        c += item.Value;
+      }
+      return c;
+    }
+
+    public IEnumerable<T> Elements {
+      get {
+        for (var i = BigInteger.Zero; i < occurrencesOfNull; i++) {
+          yield return default(T);
+        }
+        foreach (var item in dict) {
+          for (var i = BigInteger.Zero; i < item.Value; i++) {
+            yield return item.Key;
+          }
+        }
+      }
+    }
+
+    public IEnumerable<T> UniqueElements {
+      get {
+        if (!occurrencesOfNull.IsZero) {
+          yield return default(T);
+        }
+        foreach (var key in dict.Keys) {
+          if (dict[key] != 0) {
+            yield return key;
+          }
+        }
+      }
+    }
+  }
+
+  public interface IMap<out U, out V> {
+    int Count { get; }
+    long LongCount { get; }
+    ISet<U> Keys { get; }
+    ISet<V> Values { get; }
+    IEnumerable<IPair<U, V>> ItemEnumerable { get; }
+    bool Contains<G>(G t);
+    /// <summary>
+    /// Returns "true" iff "this is IMap<object, object>" and "this" equals "other".
+    /// </summary>
+    bool EqualsObjObj(IMap<object, object> other);
+    IMap<UU, VV> DowncastClone<UU, VV>(Func<U, UU> keyConverter, Func<V, VV> valueConverter);
+  }
+
+  public class Map<U, V> : IMap<U, V> {
+    readonly ImmutableDictionary<U, V> dict;
+    readonly bool hasNullKey;  // true when "null" is a key of the Map
+    readonly V nullValue;  // if "hasNullKey", the value that "null" maps to
+
+    private Map(ImmutableDictionary<U, V>.Builder d, bool hasNullKey, V nullValue) {
+      dict = d.ToImmutable();
+      this.hasNullKey = hasNullKey;
+      this.nullValue = nullValue;
+    }
+    public static readonly Map<U, V> Empty = new Map<U, V>(ImmutableDictionary<U, V>.Empty.ToBuilder(), false, default(V));
+
+    private Map(ImmutableDictionary<U, V> d, bool hasNullKey, V nullValue) {
+      dict = d;
+      this.hasNullKey = hasNullKey;
+      this.nullValue = nullValue;
+    }
+
+    private static readonly TypeDescriptor<IMap<U, V>> _TYPE = new Dafny.TypeDescriptor<IMap<U, V>>(Empty);
+    public static TypeDescriptor<IMap<U, V>> _TypeDescriptor() {
+      return _TYPE;
+    }
+
+    public static Map<U, V> FromElements(params IPair<U, V>[] values) {
+      var d = ImmutableDictionary<U, V>.Empty.ToBuilder();
+      var hasNullKey = false;
+      var nullValue = default(V);
+      foreach (var p in values) {
+        if (p.Car == null) {
+          hasNullKey = true;
+          nullValue = p.Cdr;
+        } else {
+          d[p.Car] = p.Cdr;
+        }
+      }
+      return new Map<U, V>(d, hasNullKey, nullValue);
+    }
+    public static Map<U, V> FromCollection(IEnumerable<IPair<U, V>> values) {
+      var d = ImmutableDictionary<U, V>.Empty.ToBuilder();
+      var hasNullKey = false;
+      var nullValue = default(V);
+      foreach (var p in values) {
+        if (p.Car == null) {
+          hasNullKey = true;
+          nullValue = p.Cdr;
+        } else {
+          d[p.Car] = p.Cdr;
+        }
+      }
+      return new Map<U, V>(d, hasNullKey, nullValue);
+    }
+    public static Map<U, V> FromIMap(IMap<U, V> m) {
+      return m as Map<U, V> ?? FromCollection(m.ItemEnumerable);
+    }
+    public IMap<UU, VV> DowncastClone<UU, VV>(Func<U, UU> keyConverter, Func<V, VV> valueConverter) {
+      if (this is IMap<UU, VV> th) {
+        return th;
+      } else {
+        var d = ImmutableDictionary<UU, VV>.Empty.ToBuilder();
+        foreach (var item in this.dict) {
+          var k = keyConverter(item.Key);
+          var v = valueConverter(item.Value);
+          d.Add(k, v);
+        }
+        return new Map<UU, VV>(d, this.hasNullKey, (VV)(object)this.nullValue);
+      }
+    }
+    public int Count {
+      get { return dict.Count + (hasNullKey ? 1 : 0); }
+    }
+    public long LongCount {
+      get { return dict.Count + (hasNullKey ? 1 : 0); }
+    }
+
+    public bool Equals(IMap<U, V> other) {
+      if (other == null || LongCount != other.LongCount) {
+        return false;
+      } else if (this == other) {
+        return true;
+      }
+      if (hasNullKey) {
+        if (!other.Contains(default(U)) || !object.Equals(nullValue, Select(other, default(U)))) {
+          return false;
+        }
+      }
+      foreach (var item in dict) {
+        if (!other.Contains(item.Key) || !object.Equals(item.Value, Select(other, item.Key))) {
+          return false;
+        }
+      }
+      return true;
+    }
+    public bool EqualsObjObj(IMap<object, object> other) {
+      if (!(this is IMap<object, object>) || other == null || LongCount != other.LongCount) {
+        return false;
+      } else if (this == other) {
+        return true;
+      }
+      var oth = Map<object, object>.FromIMap(other);
+      if (hasNullKey) {
+        if (!oth.Contains(default(U)) || !object.Equals(nullValue, Map<object, object>.Select(oth, default(U)))) {
+          return false;
+        }
+      }
+      foreach (var item in dict) {
+        if (!other.Contains(item.Key) || !object.Equals(item.Value, Map<object, object>.Select(oth, item.Key))) {
+          return false;
+        }
+      }
+      return true;
+    }
+    public override bool Equals(object other) {
+      // See comment in Set.Equals
+      var m = other as IMap<U, V>;
+      if (m != null) {
+        return Equals(m);
+      }
+      var imapoo = other as IMap<object, object>;
+      if (imapoo != null) {
+        return EqualsObjObj(imapoo);
+      } else {
+        return false;
+      }
+    }
+
+    public override int GetHashCode() {
+      var hashCode = 1;
+      if (hasNullKey) {
+        var key = Dafny.Helpers.GetHashCode(default(U));
+        key = (key << 3) | (key >> 29) ^ Dafny.Helpers.GetHashCode(nullValue);
+        hashCode = hashCode * (key + 3);
+      }
+      foreach (var kv in dict) {
+        var key = Dafny.Helpers.GetHashCode(kv.Key);
+        key = (key << 3) | (key >> 29) ^ Dafny.Helpers.GetHashCode(kv.Value);
+        hashCode = hashCode * (key + 3);
+      }
+      return hashCode;
+    }
+    public override string ToString() {
+      var s = "map[";
+      var sep = "";
+      if (hasNullKey) {
+        s += sep + Dafny.Helpers.ToString(default(U)) + " := " + Dafny.Helpers.ToString(nullValue);
+        sep = ", ";
+      }
+      foreach (var kv in dict) {
+        s += sep + Dafny.Helpers.ToString(kv.Key) + " := " + Dafny.Helpers.ToString(kv.Value);
+        sep = ", ";
+      }
+      return s + "]";
+    }
+    public bool Contains<G>(G u) {
+      return u == null ? hasNullKey : u is U && dict.ContainsKey((U)(object)u);
+    }
+    public static V Select(IMap<U, V> th, U index) {
+      // the following will throw an exception if "index" in not a key of the map
+      var m = FromIMap(th);
+      return index == null && m.hasNullKey ? m.nullValue : m.dict[index];
+    }
+    public static IMap<U, V> Update(IMap<U, V> th, U index, V val) {
+      var m = FromIMap(th);
+      var d = m.dict.ToBuilder();
+      if (index == null) {
+        return new Map<U, V>(d, true, val);
+      } else {
+        d[index] = val;
+        return new Map<U, V>(d, m.hasNullKey, m.nullValue);
+      }
+    }
+
+    public static IMap<U, V> Merge(IMap<U, V> th, IMap<U, V> other) {
+      var a = FromIMap(th);
+      var b = FromIMap(other);
+      ImmutableDictionary<U, V> d = a.dict.SetItems(b.dict);
+      return new Map<U, V>(d, a.hasNullKey || b.hasNullKey, b.hasNullKey ? b.nullValue : a.nullValue);
+    }
+
+    public static IMap<U, V> Subtract(IMap<U, V> th, ISet<U> keys) {
+      var a = FromIMap(th);
+      ImmutableDictionary<U, V> d = a.dict.RemoveRange(keys.Elements);
+      return new Map<U, V>(d, a.hasNullKey && !keys.Contains<object>(null), a.nullValue);
+    }
+
+    public ISet<U> Keys {
+      get {
+        if (hasNullKey) {
+          return Dafny.Set<U>.FromCollectionPlusOne(dict.Keys, default(U));
+        } else {
+          return Dafny.Set<U>.FromCollection(dict.Keys);
+        }
+      }
+    }
+    public ISet<V> Values {
+      get {
+        if (hasNullKey) {
+          return Dafny.Set<V>.FromCollectionPlusOne(dict.Values, nullValue);
+        } else {
+          return Dafny.Set<V>.FromCollection(dict.Values);
+        }
+      }
+    }
+
+    public IEnumerable<IPair<U, V>> ItemEnumerable {
+      get {
+        if (hasNullKey) {
+          yield return new Pair<U, V>(default(U), nullValue);
+        }
+        foreach (KeyValuePair<U, V> kvp in dict) {
+          yield return new Pair<U, V>(kvp.Key, kvp.Value);
+        }
+      }
+    }
+
+    public static ISet<_System.Tuple2<U, V>> Items(IMap<U, V> m) {
+      var result = new HashSet<_System.Tuple2<U, V>>();
+      foreach (var item in m.ItemEnumerable) {
+        result.Add(_System.Tuple2<U, V>.create(item.Car, item.Cdr));
+      }
+      return Dafny.Set<_System.Tuple2<U, V>>.FromCollection(result);
+    }
+  }
+
+  public interface ISequence<out T> {
+    long LongCount { get; }
+    int Count { get; }
+    T[] Elements { get; }
+    IEnumerable<T> UniqueElements { get; }
+    T Select(ulong index);
+    T Select(long index);
+    T Select(uint index);
+    T Select(int index);
+    T Select(BigInteger index);
+    bool Contains<G>(G g);
+    ISequence<T> Take(long m);
+    ISequence<T> Take(ulong n);
+    ISequence<T> Take(BigInteger n);
+    ISequence<T> Drop(long m);
+    ISequence<T> Drop(ulong n);
+    ISequence<T> Drop(BigInteger n);
+    ISequence<T> Subsequence(long lo, long hi);
+    ISequence<T> Subsequence(long lo, ulong hi);
+    ISequence<T> Subsequence(long lo, BigInteger hi);
+    ISequence<T> Subsequence(ulong lo, long hi);
+    ISequence<T> Subsequence(ulong lo, ulong hi);
+    ISequence<T> Subsequence(ulong lo, BigInteger hi);
+    ISequence<T> Subsequence(BigInteger lo, long hi);
+    ISequence<T> Subsequence(BigInteger lo, ulong hi);
+    ISequence<T> Subsequence(BigInteger lo, BigInteger hi);
+    bool EqualsAux(ISequence<object> other);
+    ISequence<U> DowncastClone<U>(Func<T, U> converter);
+  }
+
+  public abstract class Sequence<T> : ISequence<T> {
+    public static readonly ISequence<T> Empty = new ArraySequence<T>(new T[0]);
+
+    private static readonly TypeDescriptor<ISequence<T>> _TYPE = new Dafny.TypeDescriptor<ISequence<T>>(Empty);
+    public static TypeDescriptor<ISequence<T>> _TypeDescriptor() {
+      return _TYPE;
+    }
+
+    public static ISequence<T> Create(BigInteger length, System.Func<BigInteger, T> init) {
+      var len = (int)length;
+      var values = new T[len];
+      for (int i = 0; i < len; i++) {
+        values[i] = init(new BigInteger(i));
+      }
+      return new ArraySequence<T>(values);
+    }
+    public static ISequence<T> FromArray(T[] values) {
+      return new ArraySequence<T>(values);
+    }
+    public static ISequence<T> FromElements(params T[] values) {
+      return new ArraySequence<T>(values);
+    }
+    public static ISequence<char> FromString(string s) {
+      return new ArraySequence<char>(s.ToCharArray());
+    }
+    public ISequence<U> DowncastClone<U>(Func<T, U> converter) {
+      if (this is ISequence<U> th) {
+        return th;
+      } else {
+        var values = new U[this.LongCount];
+        for (long i = 0; i < this.LongCount; i++) {
+          var val = converter(this.Select(i));
+          values[i] = val;
+        }
+        return new ArraySequence<U>(values);
+      }
+    }
+    public static ISequence<T> Update(ISequence<T> sequence, long index, T t) {
+      T[] tmp = (T[])sequence.Elements.Clone();
+      tmp[index] = t;
+      return new ArraySequence<T>(tmp);
+    }
+    public static ISequence<T> Update(ISequence<T> sequence, ulong index, T t) {
+      return Update(sequence, (long)index, t);
+    }
+    public static ISequence<T> Update(ISequence<T> sequence, BigInteger index, T t) {
+      return Update(sequence, (long)index, t);
+    }
+    public static bool EqualUntil(ISequence<T> left, ISequence<T> right, int n) {
+      T[] leftElmts = left.Elements, rightElmts = right.Elements;
+      for (int i = 0; i < n; i++) {
+        if (!object.Equals(leftElmts[i], rightElmts[i]))
+          return false;
+      }
+      return true;
+    }
+    public static bool IsPrefixOf(ISequence<T> left, ISequence<T> right) {
+      int n = left.Elements.Length;
+      return n <= right.Elements.Length && EqualUntil(left, right, n);
+    }
+    public static bool IsProperPrefixOf(ISequence<T> left, ISequence<T> right) {
+      int n = left.Elements.Length;
+      return n < right.Elements.Length && EqualUntil(left, right, n);
+    }
+    public static ISequence<T> Concat(ISequence<T> left, ISequence<T> right) {
+      if (left.Count == 0) {
+        return right;
+      }
+      if (right.Count == 0) {
+        return left;
+      }
+      return new ConcatSequence<T>(left, right);
+    }
+    // Make Count a public abstract instead of LongCount, since the "array size is limited to a total of 4 billion
+    // elements, and to a maximum index of 0X7FEFFFFF". Therefore, as a protection, limit this to int32.
+    // https://docs.microsoft.com/en-us/dotnet/api/system.array
+    public abstract int Count { get; }
+    public long LongCount {
+      get { return Count; }
+    }
+    // ImmutableElements cannot be public in the interface since ImmutableArray<T> leads to a
+    // "covariant type T occurs in invariant position" error. There do not appear to be interfaces for ImmutableArray<T>
+    // that resolve this.
+    protected abstract ImmutableArray<T> ImmutableElements { get; }
+
+    public T[] Elements {
+      get { return ImmutableElements.ToArray(); }
+    }
+    public IEnumerable<T> UniqueElements {
+      get {
+        var st = Set<T>.FromCollection(ImmutableElements);
+        return st.Elements;
+      }
+    }
+
+    public T Select(ulong index) {
+      return ImmutableElements[checked((int)index)];
+    }
+    public T Select(long index) {
+      return ImmutableElements[checked((int)index)];
+    }
+    public T Select(uint index) {
+      return ImmutableElements[checked((int)index)];
+    }
+    public T Select(int index) {
+      return ImmutableElements[index];
+    }
+    public T Select(BigInteger index) {
+      return ImmutableElements[(int)index];
+    }
+    public bool Equals(ISequence<T> other) {
+      int n = ImmutableElements.Length;
+      return n == other.Elements.Length && EqualUntil(this, other, n);
+    }
+    public override bool Equals(object other) {
+      if (other is ISequence<T>) {
+        return Equals((ISequence<T>)other);
+      }
+      var th = this as ISequence<object>;
+      var oth = other as ISequence<object>;
+      if (th != null && oth != null) {
+        // see explanation in Set.Equals
+        return oth.EqualsAux(th);
+      } else {
+        return false;
+      }
+    }
+    public bool EqualsAux(ISequence<object> other) {
+      var s = other as ISequence<T>;
+      if (s != null) {
+        return Equals(s);
+      } else {
+        return false;
+      }
+    }
+    public override int GetHashCode() {
+      ImmutableArray<T> elmts = ImmutableElements;
+      // https://devblogs.microsoft.com/dotnet/please-welcome-immutablearrayt/
+      if (elmts.IsDefaultOrEmpty)
+        return 0;
+      var hashCode = 0;
+      for (var i = 0; i < elmts.Length; i++) {
+        hashCode = (hashCode << 3) | (hashCode >> 29) ^ Dafny.Helpers.GetHashCode(elmts[i]);
+      }
+      return hashCode;
+    }
+    public override string ToString() {
+      // This is required because (ImmutableElements is ImmutableArray<char>) is not a valid type check
+      var typeCheckTmp = new T[0];
+      ImmutableArray<T> elmts = ImmutableElements;
+      if (typeCheckTmp is char[]) {
+        var s = "";
+        foreach (var t in elmts) {
+          s += t.ToString();
+        }
+        return s;
+      } else {
+        var s = "[";
+        var sep = "";
+        foreach (var t in elmts) {
+          s += sep + Dafny.Helpers.ToString(t);
+          sep = ", ";
+        }
+        return s + "]";
+      }
+    }
+    public bool Contains<G>(G g) {
+      if (g == null || g is T) {
+        var t = (T)(object)g;
+        return ImmutableElements.Contains(t);
+      }
+      return false;
+    }
+    public ISequence<T> Take(long m) {
+      if (ImmutableElements.Length == m)
+        return this;
+      int length = checked((int)m);
+      T[] tmp = new T[length];
+      ImmutableElements.CopyTo(0, tmp, 0, length);
+      return new ArraySequence<T>(tmp);
+    }
+    public ISequence<T> Take(ulong n) {
+      return Take((long)n);
+    }
+    public ISequence<T> Take(BigInteger n) {
+      return Take((long)n);
+    }
+    public ISequence<T> Drop(long m) {
+      int startingElement = checked((int)m);
+      if (startingElement == 0)
+        return this;
+      int length = ImmutableElements.Length - startingElement;
+      T[] tmp = new T[length];
+      ImmutableElements.CopyTo(startingElement, tmp, 0, length);
+      return new ArraySequence<T>(tmp);
+    }
+    public ISequence<T> Drop(ulong n) {
+      return Drop((long)n);
+    }
+    public ISequence<T> Drop(BigInteger n) {
+      if (n.IsZero)
+        return this;
+      return Drop((long)n);
+    }
+    public ISequence<T> Subsequence(long lo, long hi) {
+      if (lo == 0 && hi == ImmutableElements.Length) {
+        return this;
+      }
+      int startingIndex = checked((int)lo);
+      int endingIndex = checked((int)hi);
+      var length = endingIndex - startingIndex;
+      T[] tmp = new T[length];
+      ImmutableElements.CopyTo(startingIndex, tmp, 0, length);
+      return new ArraySequence<T>(tmp);
+    }
+    public ISequence<T> Subsequence(long lo, ulong hi) {
+      return Subsequence(lo, (long)hi);
+    }
+    public ISequence<T> Subsequence(long lo, BigInteger hi) {
+      return Subsequence(lo, (long)hi);
+    }
+    public ISequence<T> Subsequence(ulong lo, long hi) {
+      return Subsequence((long)lo, hi);
+    }
+    public ISequence<T> Subsequence(ulong lo, ulong hi) {
+      return Subsequence((long)lo, (long)hi);
+    }
+    public ISequence<T> Subsequence(ulong lo, BigInteger hi) {
+      return Subsequence((long)lo, (long)hi);
+    }
+    public ISequence<T> Subsequence(BigInteger lo, long hi) {
+      return Subsequence((long)lo, hi);
+    }
+    public ISequence<T> Subsequence(BigInteger lo, ulong hi) {
+      return Subsequence((long)lo, (long)hi);
+    }
+    public ISequence<T> Subsequence(BigInteger lo, BigInteger hi) {
+      return Subsequence((long)lo, (long)hi);
+    }
+  }
+
+  internal class ArraySequence<T> : Sequence<T> {
+    private readonly ImmutableArray<T> elmts;
+
+    internal ArraySequence(ImmutableArray<T> ee) {
+      elmts = ee;
+    }
+    internal ArraySequence(T[] ee) {
+      elmts = ImmutableArray.Create<T>(ee);
+    }
+
+    protected override ImmutableArray<T> ImmutableElements {
+      get {
+        return elmts;
+      }
+    }
+    public override int Count {
+      get {
+        return elmts.Length;
+      }
+    }
+  }
+
+  internal class ConcatSequence<T> : Sequence<T> {
+    // INVARIANT: Either left != null, right != null, and elmts's underlying array == null or
+    // left == null, right == null, and elmts's underlying array != null
+    private ISequence<T> left, right;
+    private ImmutableArray<T> elmts;
+    private readonly int count;
+
+    internal ConcatSequence(ISequence<T> left, ISequence<T> right) {
+      this.left = left;
+      this.right = right;
+      this.count = left.Count + right.Count;
+    }
+
+    protected override ImmutableArray<T> ImmutableElements {
+      get {
+        // IsDefault returns true if the underlying array is a null reference
+        // https://devblogs.microsoft.com/dotnet/please-welcome-immutablearrayt/
+        if (elmts.IsDefault) {
+          elmts = ComputeElements();
+          // We don't need the original sequences anymore; let them be
+          // garbage-collected
+          left = null;
+          right = null;
+        }
+        return elmts;
+      }
+    }
+
+    public override int Count {
+      get {
+        return count;
+      }
+    }
+
+    private ImmutableArray<T> ComputeElements() {
+      // Traverse the tree formed by all descendants which are ConcatSequences
+      var ansBuilder = ImmutableArray.CreateBuilder<T>();
+      var toVisit = new Stack<ISequence<T>>();
+      toVisit.Push(right);
+      toVisit.Push(left);
+
+      while (toVisit.Count != 0) {
+        var seq = toVisit.Pop();
+        var cs = seq as ConcatSequence<T>;
+        if (cs != null && cs.elmts.IsDefault) {
+          toVisit.Push(cs.right);
+          toVisit.Push(cs.left);
+        } else {
+          var array = seq.Elements;
+          ansBuilder.AddRange(array);
+        }
+      }
+      return ansBuilder.ToImmutable();
+    }
+  }
+
+  public interface IPair<out A, out B> {
+    A Car { get; }
+    B Cdr { get; }
+  }
+
+  public class Pair<A, B> : IPair<A, B> {
+    private A car;
+    private B cdr;
+    public A Car { get { return car; } }
+    public B Cdr { get { return cdr; } }
+    public Pair(A a, B b) {
+      this.car = a;
+      this.cdr = b;
+    }
+  }
+
+  public class TypeDescriptor<T> {
+    private readonly T initValue;
+    public TypeDescriptor(T initValue) {
+      this.initValue = initValue;
+    }
+    public T Default() {
+      return initValue;
+    }
+  }
+
+  public partial class Helpers {
+    public static int GetHashCode<G>(G g) {
+      return g == null ? 1001 : g.GetHashCode();
+    }
+
+    public static int ToIntChecked(BigInteger i, string msg) {
+      if (i > Int32.MaxValue || i < Int32.MinValue) {
+        if (msg == null) msg = "value out of range for a 32-bit int";
+        throw new HaltException(msg + ": " + i);
+      }
+      return (int)i;
+    }
+    public static int ToIntChecked(long i, string msg) {
+      if (i > Int32.MaxValue || i < Int32.MinValue) {
+        if (msg == null) msg = "value out of range for a 32-bit int";
+        throw new HaltException(msg + ": " + i);
+      }
+      return (int)i;
+    }
+    public static int ToIntChecked(int i, string msg) {
+      return i;
+    }
+
+    public static string ToString<G>(G g) {
+      if (g == null) {
+        return "null";
+      } else if (g is bool) {
+        return (bool)(object)g ? "true" : "false";  // capitalize boolean literals like in Dafny
+      } else {
+        return g.ToString();
+      }
+    }
+    public static void Print<G>(G g) {
+      System.Console.Write(ToString(g));
+    }
+
+    public static readonly TypeDescriptor<bool> BOOL = new TypeDescriptor<bool>(false);
+    public static readonly TypeDescriptor<char> CHAR = new TypeDescriptor<char>('D');  // See CharType.DefaultValue in Dafny source code
+    public static readonly TypeDescriptor<BigInteger> INT = new TypeDescriptor<BigInteger>(BigInteger.Zero);
+    public static readonly TypeDescriptor<BigRational> REAL = new TypeDescriptor<BigRational>(BigRational.ZERO);
+    public static readonly TypeDescriptor<byte> UINT8 = new TypeDescriptor<byte>(0);
+    public static readonly TypeDescriptor<ushort> UINT16 = new TypeDescriptor<ushort>(0);
+    public static readonly TypeDescriptor<uint> UINT32 = new TypeDescriptor<uint>(0);
+    public static readonly TypeDescriptor<ulong> UINT64 = new TypeDescriptor<ulong>(0);
+
+    public static TypeDescriptor<T> NULL<T>() where T : class {
+      return new TypeDescriptor<T>(null);
+    }
+
+    public static TypeDescriptor<A[]> ARRAY<A>() {
+      return new TypeDescriptor<A[]>(new A[0]);
+    }
+
+    public static bool Quantifier<T>(IEnumerable<T> vals, bool frall, System.Predicate<T> pred) {
+      foreach (var u in vals) {
+        if (pred(u) != frall) { return !frall; }
+      }
+      return frall;
+    }
+    // Enumerating other collections
+    public static IEnumerable<bool> AllBooleans() {
+      yield return false;
+      yield return true;
+    }
+    public static IEnumerable<char> AllChars() {
+      for (int i = 0; i < 0x10000; i++) {
+        yield return (char)i;
+      }
+    }
+    public static IEnumerable<BigInteger> AllIntegers() {
+      yield return new BigInteger(0);
+      for (var j = new BigInteger(1); ; j++) {
+        yield return j;
+        yield return -j;
+      }
+    }
+    public static IEnumerable<BigInteger> IntegerRange(Nullable<BigInteger> lo, Nullable<BigInteger> hi) {
+      if (lo == null) {
+        for (var j = (BigInteger)hi; true;) {
+          j--;
+          yield return j;
+        }
+      } else if (hi == null) {
+        for (var j = (BigInteger)lo; true; j++) {
+          yield return j;
+        }
+      } else {
+        for (var j = (BigInteger)lo; j < hi; j++) {
+          yield return j;
+        }
+      }
+    }
+    public static IEnumerable<T> SingleValue<T>(T e) {
+      yield return e;
+    }
+    // pre: b != 0
+    // post: result == a/b, as defined by Euclidean Division (http://en.wikipedia.org/wiki/Modulo_operation)
+    public static sbyte EuclideanDivision_sbyte(sbyte a, sbyte b) {
+      return (sbyte)EuclideanDivision_int(a, b);
+    }
+    public static short EuclideanDivision_short(short a, short b) {
+      return (short)EuclideanDivision_int(a, b);
+    }
+    public static int EuclideanDivision_int(int a, int b) {
+      if (0 <= a) {
+        if (0 <= b) {
+          // +a +b: a/b
+          return (int)(((uint)(a)) / ((uint)(b)));
+        } else {
+          // +a -b: -(a/(-b))
+          return -((int)(((uint)(a)) / ((uint)(unchecked(-b)))));
+        }
+      } else {
+        if (0 <= b) {
+          // -a +b: -((-a-1)/b) - 1
+          return -((int)(((uint)(-(a + 1))) / ((uint)(b)))) - 1;
+        } else {
+          // -a -b: ((-a-1)/(-b)) + 1
+          return ((int)(((uint)(-(a + 1))) / ((uint)(unchecked(-b))))) + 1;
+        }
+      }
+    }
+    public static long EuclideanDivision_long(long a, long b) {
+      if (0 <= a) {
+        if (0 <= b) {
+          // +a +b: a/b
+          return (long)(((ulong)(a)) / ((ulong)(b)));
+        } else {
+          // +a -b: -(a/(-b))
+          return -((long)(((ulong)(a)) / ((ulong)(unchecked(-b)))));
+        }
+      } else {
+        if (0 <= b) {
+          // -a +b: -((-a-1)/b) - 1
+          return -((long)(((ulong)(-(a + 1))) / ((ulong)(b)))) - 1;
+        } else {
+          // -a -b: ((-a-1)/(-b)) + 1
+          return ((long)(((ulong)(-(a + 1))) / ((ulong)(unchecked(-b))))) + 1;
+        }
+      }
+    }
+    public static BigInteger EuclideanDivision(BigInteger a, BigInteger b) {
+      if (0 <= a.Sign) {
+        if (0 <= b.Sign) {
+          // +a +b: a/b
+          return BigInteger.Divide(a, b);
+        } else {
+          // +a -b: -(a/(-b))
+          return BigInteger.Negate(BigInteger.Divide(a, BigInteger.Negate(b)));
+        }
+      } else {
+        if (0 <= b.Sign) {
+          // -a +b: -((-a-1)/b) - 1
+          return BigInteger.Negate(BigInteger.Divide(BigInteger.Negate(a) - 1, b)) - 1;
+        } else {
+          // -a -b: ((-a-1)/(-b)) + 1
+          return BigInteger.Divide(BigInteger.Negate(a) - 1, BigInteger.Negate(b)) + 1;
+        }
+      }
+    }
+    // pre: b != 0
+    // post: result == a%b, as defined by Euclidean Division (http://en.wikipedia.org/wiki/Modulo_operation)
+    public static sbyte EuclideanModulus_sbyte(sbyte a, sbyte b) {
+      return (sbyte)EuclideanModulus_int(a, b);
+    }
+    public static short EuclideanModulus_short(short a, short b) {
+      return (short)EuclideanModulus_int(a, b);
+    }
+    public static int EuclideanModulus_int(int a, int b) {
+      uint bp = (0 <= b) ? (uint)b : (uint)(unchecked(-b));
+      if (0 <= a) {
+        // +a: a % b'
+        return (int)(((uint)a) % bp);
+      } else {
+        // c = ((-a) % b')
+        // -a: b' - c if c > 0
+        // -a: 0 if c == 0
+        uint c = ((uint)(unchecked(-a))) % bp;
+        return (int)(c == 0 ? c : bp - c);
+      }
+    }
+    public static long EuclideanModulus_long(long a, long b) {
+      ulong bp = (0 <= b) ? (ulong)b : (ulong)(unchecked(-b));
+      if (0 <= a) {
+        // +a: a % b'
+        return (long)(((ulong)a) % bp);
+      } else {
+        // c = ((-a) % b')
+        // -a: b' - c if c > 0
+        // -a: 0 if c == 0
+        ulong c = ((ulong)(unchecked(-a))) % bp;
+        return (long)(c == 0 ? c : bp - c);
+      }
+    }
+    public static BigInteger EuclideanModulus(BigInteger a, BigInteger b) {
+      var bp = BigInteger.Abs(b);
+      if (0 <= a.Sign) {
+        // +a: a % b'
+        return BigInteger.Remainder(a, bp);
+      } else {
+        // c = ((-a) % b')
+        // -a: b' - c if c > 0
+        // -a: 0 if c == 0
+        var c = BigInteger.Remainder(BigInteger.Negate(a), bp);
+        return c.IsZero ? c : BigInteger.Subtract(bp, c);
+      }
+    }
+
+    public static U CastConverter<T, U>(T t) {
+      return (U)(object)t;
+    }
+
+    public static Sequence<T> SeqFromArray<T>(T[] array) {
+      return new ArraySequence<T>((T[])array.Clone());
+    }
+    // In .NET version 4.5, it is possible to mark a method with "AggressiveInlining", which says to inline the
+    // method if possible.  Method "ExpressionSequence" would be a good candidate for it:
+    // [System.Runtime.CompilerServices.MethodImpl(System.Runtime.CompilerServices.MethodImplOptions.AggressiveInlining)]
+    public static U ExpressionSequence<T, U>(T t, U u) {
+      return u;
+    }
+
+    public static U Let<T, U>(T t, Func<T, U> f) {
+      return f(t);
+    }
+
+    public static A Id<A>(A a) {
+      return a;
+    }
+
+    public static void WithHaltHandling(Action action) {
+      try {
+        action();
+      } catch (HaltException e) {
+        Console.WriteLine("[Program halted] " + e.Message);
+      }
+    }
+  }
+
+  public class BigOrdinal {
+    public static bool IsLimit(BigInteger ord) {
+      return ord == 0;
+    }
+    public static bool IsSucc(BigInteger ord) {
+      return 0 < ord;
+    }
+    public static BigInteger Offset(BigInteger ord) {
+      return ord;
+    }
+    public static bool IsNat(BigInteger ord) {
+      return true;  // at run time, every ORDINAL is a natural number
+    }
+  }
+
+  public struct BigRational {
+    public static readonly BigRational ZERO = new BigRational(0);
+
+    // We need to deal with the special case "num == 0 && den == 0", because
+    // that's what C#'s default struct constructor will produce for BigRational. :(
+    // To deal with it, we ignore "den" when "num" is 0.
+    BigInteger num, den;  // invariant 1 <= den || (num == 0 && den == 0)
+    public override string ToString() {
+      int log10;
+      if (num.IsZero || den.IsOne) {
+        return string.Format("{0}.0", num);
+      } else if (IsPowerOf10(den, out log10)) {
+        string sign;
+        string digits;
+        if (num.Sign < 0) {
+          sign = "-"; digits = (-num).ToString();
+        } else {
+          sign = ""; digits = num.ToString();
+        }
+        if (log10 < digits.Length) {
+          var n = digits.Length - log10;
+          return string.Format("{0}{1}.{2}", sign, digits.Substring(0, n), digits.Substring(n));
+        } else {
+          return string.Format("{0}0.{1}{2}", sign, new string('0', log10 - digits.Length), digits);
+        }
+      } else {
+        return string.Format("({0}.0 / {1}.0)", num, den);
+      }
+    }
+    public bool IsPowerOf10(BigInteger x, out int log10) {
+      log10 = 0;
+      if (x.IsZero) {
+        return false;
+      }
+      while (true) {  // invariant: x != 0 && x * 10^log10 == old(x)
+        if (x.IsOne) {
+          return true;
+        } else if (x % 10 == 0) {
+          log10++;
+          x /= 10;
+        } else {
+          return false;
+        }
+      }
+    }
+    public BigRational(int n) {
+      num = new BigInteger(n);
+      den = BigInteger.One;
+    }
+    public BigRational(BigInteger n, BigInteger d) {
+      // requires 1 <= d
+      num = n;
+      den = d;
+    }
+    public BigInteger ToBigInteger() {
+      if (num.IsZero || den.IsOne) {
+        return num;
+      } else if (0 < num.Sign) {
+        return num / den;
+      } else {
+        return (num - den + 1) / den;
+      }
+    }
+    /// <summary>
+    /// Returns values such that aa/dd == a and bb/dd == b.
+    /// </summary>
+    private static void Normalize(BigRational a, BigRational b, out BigInteger aa, out BigInteger bb, out BigInteger dd) {
+      if (a.num.IsZero) {
+        aa = a.num;
+        bb = b.num;
+        dd = b.den;
+      } else if (b.num.IsZero) {
+        aa = a.num;
+        dd = a.den;
+        bb = b.num;
+      } else {
+        var gcd = BigInteger.GreatestCommonDivisor(a.den, b.den);
+        var xx = a.den / gcd;
+        var yy = b.den / gcd;
+        // We now have a == a.num / (xx * gcd) and b == b.num / (yy * gcd).
+        aa = a.num * yy;
+        bb = b.num * xx;
+        dd = a.den * yy;
+      }
+    }
+    public int CompareTo(BigRational that) {
+      // simple things first
+      int asign = this.num.Sign;
+      int bsign = that.num.Sign;
+      if (asign < 0 && 0 <= bsign) {
+        return -1;
+      } else if (asign <= 0 && 0 < bsign) {
+        return -1;
+      } else if (bsign < 0 && 0 <= asign) {
+        return 1;
+      } else if (bsign <= 0 && 0 < asign) {
+        return 1;
+      }
+      BigInteger aa, bb, dd;
+      Normalize(this, that, out aa, out bb, out dd);
+      return aa.CompareTo(bb);
+    }
+    public int Sign {
+      get {
+        return num.Sign;
+      }
+    }
+    public override int GetHashCode() {
+      return num.GetHashCode() + 29 * den.GetHashCode();
+    }
+    public override bool Equals(object obj) {
+      if (obj is BigRational) {
+        return this == (BigRational)obj;
+      } else {
+        return false;
+      }
+    }
+    public static bool operator ==(BigRational a, BigRational b) {
+      return a.CompareTo(b) == 0;
+    }
+    public static bool operator !=(BigRational a, BigRational b) {
+      return a.CompareTo(b) != 0;
+    }
+    public static bool operator >(BigRational a, BigRational b) {
+      return a.CompareTo(b) > 0;
+    }
+    public static bool operator >=(BigRational a, BigRational b) {
+      return a.CompareTo(b) >= 0;
+    }
+    public static bool operator <(BigRational a, BigRational b) {
+      return a.CompareTo(b) < 0;
+    }
+    public static bool operator <=(BigRational a, BigRational b) {
+      return a.CompareTo(b) <= 0;
+    }
+    public static BigRational operator +(BigRational a, BigRational b) {
+      BigInteger aa, bb, dd;
+      Normalize(a, b, out aa, out bb, out dd);
+      return new BigRational(aa + bb, dd);
+    }
+    public static BigRational operator -(BigRational a, BigRational b) {
+      BigInteger aa, bb, dd;
+      Normalize(a, b, out aa, out bb, out dd);
+      return new BigRational(aa - bb, dd);
+    }
+    public static BigRational operator -(BigRational a) {
+      return new BigRational(-a.num, a.den);
+    }
+    public static BigRational operator *(BigRational a, BigRational b) {
+      return new BigRational(a.num * b.num, a.den * b.den);
+    }
+    public static BigRational operator /(BigRational a, BigRational b) {
+      // Compute the reciprocal of b
+      BigRational bReciprocal;
+      if (0 < b.num.Sign) {
+        bReciprocal = new BigRational(b.den, b.num);
+      } else {
+        // this is the case b.num < 0
+        bReciprocal = new BigRational(-b.den, -b.num);
+      }
+      return a * bReciprocal;
+    }
+  }
+
+  public class HaltException : Exception {
+    public HaltException(object message) : base(message.ToString()) {
+    }
+  }
+}
+
+namespace @_System {
+  public class Tuple2<T0, T1> {
+    public readonly T0 _0;
+    public readonly T1 _1;
+    public Tuple2(T0 _0, T1 _1) {
+      this._0 = _0;
+      this._1 = _1;
+    }
+    public override bool Equals(object other) {
+      var oth = other as _System.Tuple2<T0, T1>;
+      return oth != null && object.Equals(this._0, oth._0) && object.Equals(this._1, oth._1);
+    }
+    public override int GetHashCode() {
+      ulong hash = 5381;
+      hash = ((hash << 5) + hash) + 0;
+      hash = ((hash << 5) + hash) + ((ulong)Dafny.Helpers.GetHashCode(this._0));
+      hash = ((hash << 5) + hash) + ((ulong)Dafny.Helpers.GetHashCode(this._1));
+      return (int)hash;
+    }
+    public override string ToString() {
+      string s = "";
+      s += "(";
+      s += Dafny.Helpers.ToString(this._0);
+      s += ", ";
+      s += Dafny.Helpers.ToString(this._1);
+      s += ")";
+      return s;
+    }
+    public static Tuple2<T0, T1> Default(T0 _default_T0, T1 _default_T1) {
+      return create(_default_T0, _default_T1);
+    }
+    public static Dafny.TypeDescriptor<_System.Tuple2<T0, T1>> _TypeDescriptor(Dafny.TypeDescriptor<T0> _td_T0, Dafny.TypeDescriptor<T1> _td_T1) {
+      return new Dafny.TypeDescriptor<_System.Tuple2<T0, T1>>(_System.Tuple2<T0, T1>.Default(_td_T0.Default(), _td_T1.Default()));
+    }
+    public static Tuple2<T0, T1> create(T0 _0, T1 _1) {
+      return new Tuple2<T0, T1>(_0, _1);
+    }
+    public bool is____hMake2 { get { return true; } }
+    public T0 dtor__0 {
+      get {
+        return this._0;
+      }
+    }
+    public T1 dtor__1 {
+      get {
+        return this._1;
+      }
+    }
+  }
+
+} // end of namespace _System
+namespace Dafny {
+  internal class ArrayHelpers {
+    public static T[] InitNewArray1<T>(T z, BigInteger size0) {
+      int s0 = (int)size0;
+      T[] a = new T[s0];
+      for (int i0 = 0; i0 < s0; i0++) {
+        a[i0] = z;
+      }
+      return a;
+    }
+  }
+} // end of namespace Dafny
+namespace _System {
+
+
+  public partial class nat {
+    private static readonly Dafny.TypeDescriptor<BigInteger> _TYPE = new Dafny.TypeDescriptor<BigInteger>(BigInteger.Zero);
+    public static Dafny.TypeDescriptor<BigInteger> _TypeDescriptor() {
+      return _TYPE;
+    }
+  }
+
+
+
+
+
+
+
+
+  public class Tuple0 {
+    public Tuple0() {
+    }
+    public override bool Equals(object other) {
+      var oth = other as _System.Tuple0;
+      return oth != null;
+    }
+    public override int GetHashCode() {
+      ulong hash = 5381;
+      hash = ((hash << 5) + hash) + 0;
+      return (int) hash;
+    }
+    public override string ToString() {
+      return "()";
+    }
+    private static readonly Tuple0 theDefault = create();
+    public static Tuple0 Default() {
+      return theDefault;
+    }
+    private static readonly Dafny.TypeDescriptor<_System.Tuple0> _TYPE = new Dafny.TypeDescriptor<_System.Tuple0>(_System.Tuple0.Default());
+    public static Dafny.TypeDescriptor<_System.Tuple0> _TypeDescriptor() {
+      return _TYPE;
+    }
+    public static Tuple0 create() {
+      return new Tuple0();
+    }
+    public static System.Collections.Generic.IEnumerable<Tuple0> AllSingletonConstructors {
+      get {
+        yield return Tuple0.create();
+      }
+    }
+  }
+} // end of namespace _System
+namespace _module {
+
+  public partial class Test {
+    public Test() {
+    }
+    public void testProcess1()
+    {
+      Kernel _71_kernel;
+      Kernel _nw0 = new Kernel();
+      _nw0.__ctor();
+      _71_kernel = _nw0;
+      Endokernel _72_endokernel;
+      Endokernel _nw1 = new Endokernel();
+      _nw1.__ctor(_71_kernel);
+      _72_endokernel = _nw1;
+      Instruction _73_instruction;
+      _73_instruction = @Instruction.create_Write('a', BigInteger.Zero);
+      Thread _74_thread;
+      Thread _nw2 = new Thread();
+      _nw2.__ctor(BigInteger.Zero, BigInteger.Zero, BigInteger.Zero, Dafny.Sequence<Instruction>.FromElements(_73_instruction), _72_endokernel);
+      _74_thread = _nw2;
+      Process _75_p;
+      Process _nw3 = new Process();
+      _nw3.__ctor(BigInteger.Zero, Dafny.Sequence<BigInteger>.FromElements(BigInteger.Zero, BigInteger.One, new BigInteger(2), new BigInteger(3)), _72_endokernel, _74_thread);
+      _75_p = _nw3;
+      (_75_p).exec();
+    }
+    public void _Main()
+    {
+      (this).testProcess1();
+    }
+    public static void _StaticMain() {
+      Test _76_b = new Test();
+      _76_b._Main();
+    }
+  }
+
+
+  public partial class Process {
+    public Process() {
+      this.pid = BigInteger.Zero;
+      this.memorySpace = Dafny.Sequence<BigInteger>.Empty;
+      this.endokernel = default(Endokernel);
+      this.thread = default(Thread);
+    }
+    public BigInteger pid;
+    public Dafny.ISequence<BigInteger> memorySpace;
+    public Endokernel endokernel;
+    public Thread thread;
+    public void __ctor(BigInteger pid, Dafny.ISequence<BigInteger> memorySpace, Endokernel endokernel__, Thread thread__)
+    {
+      (this).pid = pid;
+      (this).memorySpace = memorySpace;
+      (this).endokernel = endokernel__;
+      (this).thread = thread__;
+    }
+    public void exec()
+    {
+      (this.thread).exec();
+    }
+  }
+
+  public partial class Endokernel {
+    public Endokernel() {
+      this.capabilities = Dafny.Map<Capability, Endoprocess>.Empty;
+      this.endoprocesses = Dafny.Map<BigInteger, Endoprocess>.Empty;
+      this.instructionMap = Dafny.Map<Instruction, Capability>.Empty;
+      this.nextPid = BigInteger.Zero;
+      this.kernel = default(Kernel);
+    }
+    public Dafny.IMap<Capability,Endoprocess> capabilities;
+    public Dafny.IMap<BigInteger,Endoprocess> endoprocesses;
+    public Dafny.IMap<Instruction,Capability> instructionMap;
+    public BigInteger nextPid;
+    public Kernel kernel;
+    public Endoprocess createEndoprocess(Capability capability, Instruction instruction)
+    {
+      Endoprocess endoprocess = default(Endoprocess);
+      Endoprocess _nw4 = new Endoprocess();
+      _nw4.__ctor(this.nextPid, capability.subspace, instruction, this);
+      endoprocess = _nw4;
+      (this).capabilities = Dafny.Map<Capability, Endoprocess>.Update(this.capabilities, capability, endoprocess);
+      (this).endoprocesses = Dafny.Map<BigInteger, Endoprocess>.Update(this.endoprocesses, this.nextPid, endoprocess);
+      (this).nextPid = (this.nextPid) + (BigInteger.One);
+      return endoprocess;
+    }
+    public void trap(Instruction instruction)
+    {
+      if (!(this.instructionMap).Contains((instruction))) {
+        Dafny.Helpers.Print(Dafny.Sequence<char>.FromString("trap error: no policy for this instruction\n"));
+      } else {
+        Capability _77_capability;
+        _77_capability = Dafny.Map<Instruction, Capability>.Select(this.instructionMap,instruction);
+        Endoprocess _78_endoprocess = default(Endoprocess);
+        if (!(this.capabilities).Contains((_77_capability))) {
+          Endoprocess _out0;
+          _out0 = (this).createEndoprocess(_77_capability, instruction);
+          _78_endoprocess = _out0;
+        } else {
+          _78_endoprocess = Dafny.Map<Capability, Endoprocess>.Select(this.capabilities,_77_capability);
+        }
+        Dafny.Helpers.Print(Dafny.Sequence<char>.FromString("Trapping instruction"));
+        Dafny.Helpers.Print(instruction);
+        Dafny.Helpers.Print(Dafny.Sequence<char>.FromString("from Process in Endokernel\n"));
+        (_78_endoprocess).exec(instruction);
+      }
+    }
+    public void trapEndoprocess(Instruction instruction, BigInteger endoId)
+    {
+      if (!(this.instructionMap).Contains((instruction))) {
+        Dafny.Helpers.Print(Dafny.Sequence<char>.FromString("trapEndoprocess error: no policy for this instruction\n"));
+      } else {
+        Capability _79_capability;
+        _79_capability = Dafny.Map<Instruction, Capability>.Select(this.instructionMap,instruction);
+        if (!(this.capabilities).Contains((_79_capability))) {
+          Dafny.Helpers.Print(Dafny.Sequence<char>.FromString("trapEndoprocess error: this endoprocess has not the required rights for such instruction\n"));
+        } else {
+          Endoprocess _80_endoprocessExpected;
+          _80_endoprocessExpected = Dafny.Map<Capability, Endoprocess>.Select(this.capabilities,_79_capability);
+          if (!(this.endoprocesses).Contains((endoId))) {
+            Dafny.Helpers.Print(Dafny.Sequence<char>.FromString("trapEndoprocess error: unknown endoprocess\n"));
+          } else {
+            Endoprocess _81_endoprocessTrapped;
+            _81_endoprocessTrapped = Dafny.Map<BigInteger, Endoprocess>.Select(this.endoprocesses,endoId);
+            if ((_81_endoprocessTrapped) != (object) (_80_endoprocessExpected)) {
+              Dafny.Helpers.Print(Dafny.Sequence<char>.FromString("trapEndoprocess error: unknown endoprocess\n"));
+            } else {
+              Dafny.Helpers.Print(Dafny.Sequence<char>.FromString("Trapping back instruction from Endoprocess in Endokernel\n"));
+              (this.kernel).exec(instruction);
+            }
+          }
+        }
+      }
+    }
+    public void __ctor(Kernel kernel)
+    {
+      (this).nextPid = BigInteger.Zero;
+      (this).capabilities = Dafny.Map<Capability, Endoprocess>.FromElements();
+      (this).endoprocesses = Dafny.Map<BigInteger, Endoprocess>.FromElements();
+      Capability _82_capability;
+      Capability _nw5 = new Capability();
+      _nw5.__ctor();
+      _82_capability = _nw5;
+      Instruction _83_instruction;
+      _83_instruction = @Instruction.create_Write('a', BigInteger.Zero);
+      (this).instructionMap = Dafny.Map<Instruction, Capability>.FromElements(new Dafny.Pair<Instruction, Capability>(_83_instruction, _82_capability));
+      (this).kernel = kernel;
+    }
+  }
+
+  public partial class Endoprocess {
+    public Endoprocess() {
+      this.id = BigInteger.Zero;
+      this.memorySpace = Dafny.Sequence<BigInteger>.Empty;
+      this.instructions = Instruction.Default();
+      this.endokernel = default(Endokernel);
+    }
+    public BigInteger id;
+    public Dafny.ISequence<BigInteger> memorySpace;
+    public Instruction instructions;
+    public Endokernel endokernel;
+    public void __ctor(BigInteger id, Dafny.ISequence<BigInteger> memorySpace, Instruction instructions, Endokernel endokernel)
+    {
+      (this).id = id;
+      (this).memorySpace = memorySpace;
+      (this).instructions = instructions;
+      (this).endokernel = endokernel;
+    }
+    public void exec(Instruction instruction)
+    {
+      Dafny.Helpers.Print(Dafny.Sequence<char>.FromString("Executing instruction in Endoprocess\n"));
+      (this.endokernel).trapEndoprocess(instruction, this.id);
+    }
+  }
+
+  public partial class Kernel {
+    public Kernel() {
+    }
+    public void exec(Instruction instruction)
+    {
+      Dafny.Helpers.Print(Dafny.Sequence<char>.FromString("Executing instruction in kernel\n"));
+    }
+    public void __ctor()
+    {
+    }
+  }
+
+  public partial class Thread {
+    public Thread() {
+      this.tid = BigInteger.Zero;
+      this.pc = BigInteger.Zero;
+      this.sp = BigInteger.Zero;
+      this.instructions = Dafny.Sequence<Instruction>.Empty;
+      this.endokernel = default(Endokernel);
+    }
+    public BigInteger tid;
+    public BigInteger pc;
+    public BigInteger sp;
+    public Dafny.ISequence<Instruction> instructions;
+    public Endokernel endokernel;
+    public void __ctor(BigInteger tid, BigInteger pc, BigInteger sp, Dafny.ISequence<Instruction> instructions, Endokernel endokernel)
+    {
+      (this).tid = tid;
+      (this).pc = pc;
+      (this).sp = sp;
+      (this).instructions = instructions;
+      (this).endokernel = endokernel;
+    }
+    public void exec()
+    {
+      if (((this.pc).Sign != -1) && ((this.pc) < (new BigInteger((this.instructions).Count)))) {
+        Dafny.Helpers.Print(Dafny.Sequence<char>.FromString("Executing instruction in Process\n"));
+        (this.endokernel).trap((this.instructions).Select(this.pc));
+        (this).pc = (this.pc) + (BigInteger.One);
+      }
+    }
+  }
+
+  public abstract class Instruction {
+    public Instruction() { }
+    private static readonly Instruction theDefault = create_Write('D', BigInteger.Zero);
+    public static Instruction Default() {
+      return theDefault;
+    }
+    private static readonly Dafny.TypeDescriptor<Instruction> _TYPE = new Dafny.TypeDescriptor<Instruction>(Instruction.Default());
+    public static Dafny.TypeDescriptor<Instruction> _TypeDescriptor() {
+      return _TYPE;
+    }
+    public static Instruction create_Write(char @value, BigInteger addr) {
+      return new Instruction_Write(@value, addr);
+    }
+    public static Instruction create_Read(BigInteger addr) {
+      return new Instruction_Read(addr);
+    }
+    public bool is_Write { get { return this is Instruction_Write; } }
+    public bool is_Read { get { return this is Instruction_Read; } }
+    public char dtor_value {
+      get {
+        var d = this;
+        return ((Instruction_Write)d).@value; 
+      }
+    }
+    public BigInteger dtor_addr {
+      get {
+        var d = this;
+        if (d is Instruction_Write) { return ((Instruction_Write)d).addr; }
+        return ((Instruction_Read)d).addr; 
+      }
+    }
+  }
+  public class Instruction_Write : Instruction {
+    public readonly char @value;
+    public readonly BigInteger addr;
+    public Instruction_Write(char @value, BigInteger addr) {
+      this.@value = @value;
+      this.addr = addr;
+    }
+    public override bool Equals(object other) {
+      var oth = other as Instruction_Write;
+      return oth != null && this.@value == oth.@value && this.addr == oth.addr;
+    }
+    public override int GetHashCode() {
+      ulong hash = 5381;
+      hash = ((hash << 5) + hash) + 0;
+      hash = ((hash << 5) + hash) + ((ulong)Dafny.Helpers.GetHashCode(this.@value));
+      hash = ((hash << 5) + hash) + ((ulong)Dafny.Helpers.GetHashCode(this.addr));
+      return (int) hash;
+    }
+    public override string ToString() {
+      string s = "Instruction.Write";
+      s += "(";
+      s += Dafny.Helpers.ToString(this.@value);
+      s += ", ";
+      s += Dafny.Helpers.ToString(this.addr);
+      s += ")";
+      return s;
+    }
+  }
+  public class Instruction_Read : Instruction {
+    public readonly BigInteger addr;
+    public Instruction_Read(BigInteger addr) {
+      this.addr = addr;
+    }
+    public override bool Equals(object other) {
+      var oth = other as Instruction_Read;
+      return oth != null && this.addr == oth.addr;
+    }
+    public override int GetHashCode() {
+      ulong hash = 5381;
+      hash = ((hash << 5) + hash) + 1;
+      hash = ((hash << 5) + hash) + ((ulong)Dafny.Helpers.GetHashCode(this.addr));
+      return (int) hash;
+    }
+    public override string ToString() {
+      string s = "Instruction.Read";
+      s += "(";
+      s += Dafny.Helpers.ToString(this.addr);
+      s += ")";
+      return s;
+    }
+  }
+
+  public partial class Capability {
+    public Capability() {
+      this.subspace = Dafny.Sequence<BigInteger>.Empty;
+      this.stack = Dafny.Sequence<BigInteger>.Empty;
+      this.files = Dafny.Sequence<Dafny.ISequence<char>>.Empty;
+      this.entries = Dafny.Sequence<Dafny.ISequence<char>>.Empty;
+    }
+    public Dafny.ISequence<BigInteger> subspace;
+    public Dafny.ISequence<BigInteger> stack;
+    public Dafny.ISequence<Dafny.ISequence<char>> files;
+    public Dafny.ISequence<Dafny.ISequence<char>> entries;
+    public void __ctor()
+    {
+      (this).subspace = Dafny.Sequence<BigInteger>.FromElements();
+      (this).stack = Dafny.Sequence<BigInteger>.FromElements();
+      (this).files = Dafny.Sequence<Dafny.ISequence<char>>.FromElements();
+      (this).entries = Dafny.Sequence<Dafny.ISequence<char>>.FromElements();
+    }
+  }
+} // end of namespace _module
+class __CallToMain {
+  public static void Main(string[] args) {
+    Dafny.Helpers.WithHaltHandling(_module.Test._StaticMain);
+  }
+}
