src/dafny/Endo.dfy
@@ -1,21 +1,22 @@
 include "Capability.dfy"
 include "Kernel.dfy"
+include "Instructions.dfy"
 
 class Endokernel {
     var capabilities: map<Capability, Endoprocess>
     var endoprocesses: map<int, Endoprocess>
-    var instructionMap: map<string, Capability>
+    var instructionMap: map<Instruction, Capability>
     var nextPid:int;
     var kernel:Kernel;
 
-    method createEndoprocess(capability:Capability, instruction:string) returns (endoprocess:Endoprocess) modifies this {
+    method createEndoprocess(capability:Capability, instruction:Instruction) returns (endoprocess:Endoprocess) modifies this {
         endoprocess := new Endoprocess(this.nextPid, capability.subspace, instruction, this);
         this.capabilities := capabilities[capability := endoprocess];
         this.endoprocesses := this.endoprocesses[this.nextPid := endoprocess];
         this.nextPid := nextPid + 1;
     }
 
-    method trap(instruction:string) modifies this  { 
+    method trap(instruction:Instruction) modifies this  { 
         if (instruction !in instructionMap){
            print "trap error: no policy for this instruction\n";
         } 
@@ -27,12 +28,15 @@ class Endokernel {
             } else {
                 endoprocess := capabilities[capability];
             }
-            print "Trapping instruction " + instruction + " from Process in Endokernel\n";
+            
+            print "Trapping instruction";
+            print instruction;
+            print "from Process in Endokernel\n";
             endoprocess.exec(instruction);
         }
     }
 
-    method trapEndoprocess(instruction:string, endoId:int) {
+    method trapEndoprocess(instruction:Instruction, endoId:int) {
         // Verifying if endoprocess has correct access rights to execute this instruction
         if (instruction !in instructionMap){
            print "trapEndoprocess error: no policy for this instruction\n";
@@ -52,7 +56,7 @@ class Endokernel {
                         print "trapEndoprocess error: unknown endoprocess\n";
                     }
                     else {
-                        print "Trapping back instruction " + instruction + " from Endoprocess in Endokernel\n";
+                        print "Trapping back instruction from Endoprocess in Endokernel\n";
                         kernel.exec(instruction);
                     }
                 }
@@ -66,7 +70,8 @@ class Endokernel {
         this.capabilities := map[];
         this.endoprocesses := map[];
         var capability:Capability := new Capability();
-        this.instructionMap := map["write(0,a)" := capability];
+        var instruction:Instruction := Write('a', 0);
+        this.instructionMap := map[instruction := capability];
         this.kernel := kernel;
     }
 }
@@ -74,18 +79,18 @@ class Endokernel {
 class Endoprocess {
     var id:int;
     var memorySpace:seq<int>
-    var instructions: string
+    var instructions: Instruction
     var endokernel:Endokernel;
 
-    constructor(id:int, memorySpace:seq<int>, instructions:string, endokernel:Endokernel) {
+    constructor(id:int, memorySpace:seq<int>, instructions:Instruction, endokernel:Endokernel) {
         this.id := id;
         this.memorySpace := memorySpace;
         this.instructions := instructions;
         this.endokernel := endokernel;
     }
 
-    method exec(instruction:string)  {
-        print "Executing instruction " + instruction + " in Endoprocess\n";
+    method exec(instruction:Instruction)  {
+        print "Executing instruction in Endoprocess\n";
         endokernel.trapEndoprocess(instruction, this.id);
     }
 }
