src/dafny/Process.dfy
@@ -4,18 +4,17 @@ include "Thread.dfy"
 class Process {
     var pid:int;
     var memorySpace: seq<int>; 
-    var instructions: seq<string>;
     var endokernel: Endokernel;
     var thread: Thread;
 
-    constructor(pid:int, memorySpace:seq<int>, instructions:seq<string>, endokernel:Endokernel)
-    ensures this.endokernel == old(endokernel)
+    constructor(pid:int, memorySpace:seq<int>, endokernel_:Endokernel, thread_:Thread)
+    ensures this.endokernel == old(endokernel_);
+    ensures this.thread == old(thread_);
     {
         this.pid := pid;
         this.memorySpace := memorySpace;
-        this.instructions := instructions;
-        this.endokernel := endokernel;
-        this.thread := new Thread(0, 0, 0, instructions, endokernel);
+        this.endokernel := endokernel_;
+        this.thread := thread_;
     }
 
     method exec() modifies this, thread, thread.endokernel {
