src/dafny/test.dfy
@@ -1,6 +1,8 @@
 include "Process.dfy"
 include "Endo.dfy"
 include "Kernel.dfy"
+include "Thread.dfy"
+include "Instructions.dfy"
 
 class Test {
 
@@ -8,18 +10,21 @@ class Test {
         // Example of a simple execution of the Endokernel abstraction
         var kernel:Kernel := new Kernel();
         var endokernel:Endokernel := new Endokernel(kernel);
-        var instruction:string := "write(0,a)";
-        var p:Process := new Process(0, [0,1,2,3], [instruction], endokernel);
+        var instruction:Instruction := Write('a', 0);
+        var thread:Thread := new Thread(0, 0, 0, [instruction], endokernel);
+        var p:Process := new Process(0, [0,1,2,3], endokernel, thread);
+        p.exec();
     }
 
-    method testProcess2() {
+/*     method testProcess2() {
         // Example of a simple execution of the Endokernel abstraction that is not handled
         var kernel:Kernel := new Kernel();
         var endokernel:Endokernel := new Endokernel(kernel);
         var instruction:string := "read(0,a)";
-        var p:Process := new Process(0, [0,1,2,3], [instruction], endokernel);
+        var thread:Thread := new Thread(0, 0, 0, [instruction], endokernel);
+        var p:Process := new Process(0, [0,1,2,3], endokernel, thread);
     }
-
+ */
 
     method Main()  {
         testProcess1();
